updating

specParCurrent/Independence.v
@@ -1,19 +1,51 @@
 Require Import Spec.
+Require Import sets. 
 Require Import Coq.Sets.Ensembles. 
 Require Import Heap. 
 
+Hint Unfold Ensembles.In Add. 
+Hint Constructors Singleton Couple Union. 
 
+Theorem InAdd : forall (T:Type) S s, Ensembles.In T (Add T S s) s. 
+Proof.  intros. unfold Add. unfold Ensembles.In. apply Union_intror. 
+  unfold Ensembles.In. apply In_singleton. 
 
-Theorem eqImpliesSameSet : forall (T:Type) T1 T2, T1 = T2 -> Same_set T T1 T2. 
+Theorem SingletonEq : forall (T:Type) e e', Singleton T e = Singleton T e' -> e = e'.
 Proof.
-  intros. unfold Same_set. unfold Included. split; intros. 
-  {subst. assumption. }
-  {subst. assumption. }
-Qed. 
+  intros. apply eqImpliesSameSet in H. unfold Same_set in H. unfold Included in H. 
+  inversion H. assert(Ensembles.In T (Singleton T e) e). auto. apply H0 in H2. 
+  inversion H2. reflexivity. Qed. 
+
+Ltac invertSetEq := 
+  match goal with
+      |H : Empty_set ?T = Singleton ?T ?e |- _ => 
+       apply eqImpliesSameSet in H; unfold Same_set in H; unfold Included in H;
+       inversion H as [sameSet1 sameSet2]; 
+       assert(Hin:Ensembles.In T (Singleton T e) e) by auto;
+       apply sameSet2 in Hin; inversion Hin
+      |H : Empty_set ?T = Couple ?T ?e1 ?e2 |- _ =>
+       apply eqImpliesSameSet in H; unfold Same_set in H; unfold Included in H;
+       inversion H as [sameSet1 sameSet2];
+       assert(Hin:Ensembles.In T (Couple T e1 e2) e1) by auto; apply sameSet2 in Hin;
+       inversion Hin
+      |H:Singleton ?T ?e = Empty_set ?T |- _ => symmetry in H; invertSetEq
+      |H:Couple ?T ?e1 ?e2 = Empty_set ?T |- _ => symmetry in H; invertSetEq
+      |H:Singleton ?T ?e1 = Couple ?T ?e2 ?e3 |- _ => apply SingleEqCouple in H
+      |H:Couple ?T ?e2 ?e3 = Singleton ?T ?e1 |- _ => symmetry in H; invertSetEq
+      |H : Empty_set ?T = Add ?T ?S ?s |- _ => 
+       apply eqImpliesSameSet in H; unfold Same_set in H; unfold Included in H; 
+       inversion H as [sameSet1 sameSet2]; assert(Hin:Ensembles.In T (Add T S s) s) by apply InAdd;
+       apply sameSet2 in Hin; inversion Hin
+      |H : Add ?T ?S ?s = Empty_set ?T |- _ => symmetry in H; invertSetEq
+      |H : Singleton ?T ?e = Singleton ?T ?e' |- _ => apply SingletonEq in H
+  end. 
+
+Ltac unfoldSetOp := repeat(try unfold tAdd in *; try unfold tIn in *; try unfold tCouple in *;
+                           try unfold tSingleton in *; try unfold tEmptySet in *).
 
 Theorem UnionEq : forall T t1 t2, tIntersection T t1 = tEmptySet -> tIntersection T t2 = tEmptySet -> 
                                   tUnion T t1 = tUnion T t2 -> t1 = t2.
-Proof.
+Proof. 
   intros. apply eqImpliesSameSet in H1. unfold Same_set in H1. inversion H1. 
   unfold Included in *. apply Extensionality_Ensembles. unfold Same_set. unfold Included. split. 
   {intros. assert(tIn (tUnion T t1) x). apply Union_intror. assumption. 
@@ -132,6 +164,21 @@ Hint Constructors Singleton.
             inversion H as [sameSet1 sameSet2]; assert(Assump:tIn (tCouple t1 t2) t1) by apply Couple_l;
             apply sameSet2 in Assump; inversion Assump
        end.
+
+Ltac setNeq :=
+  unfold tAdd in *; 
+  match goal with
+      |H:Empty_set ?T = Add ?T ?S ?s |- _ =>
+       apply eqImpliesSameSet in H; unfold Same_set in H; unfold Included in H;
+       inversion H as [sameSet1 sameSet2]; assert(Assump:In T (Add T S s) s) by auto;
+       apply sameSet2 in Assump; inversion Assump
+      |H:Empty_set ?T = Couple ?T ?t1 ?t2 |- _ =>
+       apply eqImpliesSameSet in H; unfold Same_set in H; unfold Included in H; 
+       inversion H as [sameSet1 sameSet2]; assert(Assump:In T (Couple T t1 t2) t1) by apply Couple_l;
+       apply sameSet2 in Assump; inversion Assump
+  end.
+                                                        
+
 Unset Ltac Debug. 
 
 Theorem AddEqIn : forall T t T', tAdd T t = T' -> tIn T' t. 
@@ -144,13 +191,25 @@ Proof.
   intros. unfoldSetEq. assert(tIn (tAdd T e2) e2) by auto. apply H1 in H2. 
   inversion H2. reflexivity. Qed. 
 
+Axiom eqSA : forall T1 T2 sa,
+               specActions T1 sa -> specActions T2 sa ->
+              (forall tid t t', thread_lookup T1 tid t -> thread_lookup T2 tid t') /\
+              (forall tid t t', thread_lookup T2 tid t -> thread_lookup T1 tid t'). 
 
-Ltac evalSpecActions :=
-  match goal with
-      |H:specActions (tCouple (Tid(?maj,?min) ?t, ?s1, ?s2, ?M)
-                              (Tid(?maj',?min') ?t', ?s1', ?s2', ?M')) ?a |- _ =>
-       assert(a = Couple (tid*specStack) (Tid(maj,0)t, s1) (Tid (maj',0)t', s1'))by admit
-  end.       
+
+Theorem InWeakening : forall T e1 e2 tid, thread_lookup T tid e1 -> thread_lookup (tAdd T e2) tid e1. 
+Proof.
+  intros. inversion H. econstructor. subst. unfold tAdd. unfold Add. 
+  apply Union_introl. assumption. eassumption. Qed. 
+
+Theorem invertTIDLookup : forall tid T e e', thread_lookup (tAdd T e) tid e' ->
+                                             thread_lookup T tid e' \/ 
+                                             thread_lookup (tSingleton e) tid e'. 
+Proof.
+  intros. inversion H. subst. inversion H0; subst. 
+  {left. econstructor. assumption. reflexivity. }
+  {right. econstructor. assumption. reflexivity. }
+Qed. 
 
 Theorem Reorder : forall T t1 t2 t1' t2' h h' sa ca,
                     specActions t2 sa -> specActions t2' sa ->
@@ -184,7 +243,7 @@ Proof.
   {inversion H4; eauto. 
    {subst. assert(t2 = t2'); eauto. contradiction. }
   }
-  {inversion H4; eauto; try(subst; eapply AddSpecAction in H; inversion H; eassumption).
+  {Case "t1 does a read". inversion H4; eauto; try(subst; eapply AddSpecAction in H; inversion H; eassumption).
    {subst. assert(t2 = t2'); eauto. contradiction. }
    {subst. eapply addSpecAction in H. inversion H. eassumption. }
    {subst. eapply addSpecAction in H. inversion H. eassumption. }
@@ -228,7 +287,7 @@ Proof.
   }
   {inversion H4; eauto. 
    {subst. assert(t2 = t2'); eauto. contradiction. }
-   {handleReadWrite. contradiction. intros contra. inversion contra. apply listNeq in H24. assumption. }
+   {handleReadWrite. contradiction. intros contra. inversion contra. apply listNeq in H26. assumption. }
    {handleReadWrite. contradiction. intros contra. inversion contra. }
    {subst. eapply addSpecAction in H. inversion H. eassumption. }
    {subst. admit. }
@@ -257,17 +316,101 @@ Proof.
   } 
 Qed. 
 
+
 Inductive multistep : sHeap -> pool -> pool -> sHeap -> pool -> pool -> Prop :=
 |multi_refl : forall h p1 p2, multistep h p1 p2 h p1 p2
 |multi_step : forall h h' h'' p1 p1' p1'' p2 p2' p2'',
                 step h p1 p2 h' p1' p2' -> multistep h' p1' p2' h'' p1'' p2'' ->
                 multistep h p1 p2 h'' p1'' p2''.
+
+Inductive multistep2 : sHeap -> pool -> pool -> sHeap -> pool -> pool -> Prop :=
+|multi_refl2 : forall h p1 p2, multistep2 h p1 p2 h p1 p2
+|multi_step2 : forall T1 T2 P1 P2 P1' P2' T2' H H' H'',
+                 T2 = tUnion P1 P2 -> Disjoint thread P1 P2 -> step H (tUnion T1 P1) P2 H' (tUnion T1 P1') P2' ->
+                 multistep2 H' T1 (tUnion P1' P2') H'' T1 T2' ->
+                 multistep2 H T1 T2 H'' T1 T2'
+.
+
 Require Import Coq.Program.Equality. 
+
+Inductive untouched : pool -> sHeap -> pool -> pool -> sHeap -> pool -> pool -> Prop :=
+  |UntouchedRefl : forall t1 h T t2, untouched t1 h T t2 h T t2
+  |UntouchedStep : forall t1 T T' T'' t2 t2' t2'' h h' h'',
+                     Included thread t1 T -> Included thread t1 T'->
+                     step h T t2 h' T' t2' -> multistep h' T' t2' h'' T'' t2'' ->
+                     untouched t1 h' T' t2' h'' T'' t2'' -> untouched t1 h T t2 h'' T'' t2''
+.
+
+Theorem multistepUntouched : forall h T t h' T' t' t1,
+                               multistep h (tUnion T t1) t h' (tUnion T' t1) t' ->
+                               untouched t1 h (tUnion T t1) t h' (tUnion T' t1) t'. 
+Proof.
+  intros. induction H. 
+  {constructor. }
+  {
+
+
+
+
+
+
+Theorem ReorderStepStar : forall t1 t2 t1' t2' h h' sa ca,
+                            specActions t2 sa -> specActions t2' sa ->
+                            commitActions t2 ca -> commitActions t2 ca ->
+                            step h t1 t2 h t1 t2' ->
+                            multistep2 h t2' t1 h' t2' t1' ->
+                            multistep2 h t2 t1 h' t2 t1' /\
+                            step h' t1' t2 h' t1' t2'. 
+Proof.
+  intros. 
+  induction H4. 
+  {split. constructor. assumption. }
+  {split. 
+   {subst. 
+
+
+Theorem ReorderStepStar : forall T t1 t2 t1' t2' h h' sa ca,
+                            specActions t2 sa -> specActions t2' sa ->
+                            commitActions t2 ca -> commitActions t2 ca ->
+                            step h (tUnion T t1) t2 h (tUnion T t1) t2' ->
+                            multistep h (tUnion T t2') t1 h' (tUnion T t2') t1' ->
+                            multistep h (tUnion T t2) t1 h' (tUnion T t2) t1' /\
+                            step h' (tUnion T t1') t2 h' (tUnion T t1') t2'. 
+Proof.
+  intros. remember (tUnion T t2'). generalize dependent t2'. induction H4. 
+  {intros. split. constructor. assumption. }
+  {intros. split. 
+   {subst. 
+
+
+Theorem EvalCtxtNeq : forall E e1 e2, e1 <> e2 -> ctxt E -> E e1 = E e2 -> False. 
+Proof.
+  intros. unfold not in *. intros. induction H0. 
+  {inversion H1. apply IHctxt in H3. assumption. }
+  {inversion H1. apply H in H3. assumption. }
+  {inversion H1. apply H in H3. assumption. }
+  {apply IHctxt in H1. assumption. }
+Qed. 
+
+
+Ltac termNeq := 
+  match goal with
+    |H: ?E ?x = ?E ?y |- _ => eapply EvalCtxtNeq with (e1 := x) (e2 := y);
+                             [intros contra; inversion contra |eassumption| assumption]
+  end.
 
 Theorem stepNoProgress : forall h T t,
                            step h T t h T t -> False. 
 Proof.
-  Admitted. 
+  intros. inversion H; try(subst; unfoldSetOp; invertSetEq; inversion H0; termNeq).  
+  {unfold not in H7. apply H7. reflexivity. }  
+  {subst. unfoldSetOp. invertSetEq. inversion H0. inversion H2. termNeq. }
+  {eapply heapUpdateNeq in H2. unfold not in H2. apply H2. eassumption. 
+   intros c. inversion c. apply listNeq in H10. assumption. }
+  {unfoldSetOp. invertSetEq. inversion H0. termNeq. }
+  {unfoldSetOp. invertSetEq. inversion H0. inversion H9. termNeq. }
+Admitted. 
+
 
 Theorem ReorderStepStar : forall T t1 t2 t1' t2' h h' sa ca,
                             specActions t2 sa -> specActions t2' sa ->
@@ -279,7 +422,10 @@ Theorem ReorderStepStar : forall T t1 t2 t1' t2' h h' sa ca,
 Proof.
   intros. induction H4. 
   {split. constructor. assumption. }
-  {
+  {split. 
+   {eapply multi_step with (h' := h') (p1' := p1') (p2' := p2').
+
+
 
 Theorem ReorderStepStar : forall T t1 t2 t1' t2' h h' sa ca,
                             specActions t2 sa -> specActions t2' sa ->
